coq/theories/ITree/Delay.v
@@ -1,7 +1,4 @@
-Require Import Coq.Program.Equality.
-Import EqNotations.
-
-From OGS Require Import Utils.
+From OGS Require Import Prelude.
 From OGS.Game Require Import Event.
 From OGS.ITree Require Import ITree.
 
@@ -15,6 +12,7 @@ Definition emb_delay {I} {E : event I I} {X i} : delay X -> itree E (X @ i) i :=
          | VisF e k => match e with end
          end).
 
+(*
 Definition subst_delay {I} {E : event I I} {X Y i} (f : X -> itree E Y i)
            : delay X -> itree E Y i :=
   cofix _subst_delay x :=
@@ -23,7 +21,21 @@ Definition subst_delay {I} {E : event I I} {X Y i} (f : X -> itree E Y i)
        | TauF t => TauF (_subst_delay t)
        | VisF e k => match e with end
        end).  
+*)
+
+From OGS.ITree Require Import Monad.
+
+Definition ret_delay {X} : X -> delay X := fun x => Ret' x .
+
+Definition tau_delay {X} : delay X -> delay X :=
+  fun t => go (TauF (t : itree ∅ₑ (fun _ : T1 => X) T1_0)) .
 
 Definition bind_delay {I} {E : event I I} {X Y i}
   : delay X -> (X -> itree E Y i) -> itree E Y i
-  := fun x f => subst_delay f x .
+  := fun x f => bind (emb_delay x) (fun _ '(Fib x) => f x) .
+
+Definition fmap_delay {X Y} (f : X -> Y) : delay X -> delay Y :=
+  fmap (fun 'T1_0 => f) T1_0 .
+
+Definition iter_delay {X Y} : (X -> delay (X + Y)) -> X -> delay Y :=
+  fun f => iter (fun 'T1_0 => f) T1_0 .
