coq/theories/ITree/Eq.v
@@ -1,8 +1,8 @@
 Require Import Coq.Program.Equality.
 From Coinduction Require Import lattice rel coinduction tactics.
 
-From OGS Require Import Utils.
-From OGS.Utils Require Import Rel.
+From OGS Require Import Prelude.
+From OGS.Utils Require Import Psh Rel.
 From OGS.Game Require Import Event.
 From OGS.ITree Require Import ITree.
 
