coq/theories/Utils.v
@@ -1,7 +1,0 @@
-Set Primitive Projections.
-
-Set Primitive Projections.
-From Equations Require Export Equations.
-Set Equations Transparent.
-
-From OGS.Utils Require Export Prelude Psh.
